theories/H10/Fractran/fractran_dio.v
@@ -13,11 +13,17 @@
 
 Require Import List Arith Omega.
 
+From Undecidability.Shared.Libs.DLW.Utils 
+  Require Import utils_tac utils_list sums rel_iter gcd.
 
-From Undecidability.Shared.Libs.DLW.Utils Require Import utils_tac utils_list sums rel_iter.
-From Undecidability.Shared.Libs.DLW.Vec Require Import pos vec.
-From Undecidability.H10.Fractran Require Import fractran_defs prime_seq.
-From Undecidability.H10.Dio Require Import dio_logic dio_bounded dio_rt_closure dio_single.
+From Undecidability.Shared.Libs.DLW.Vec 
+  Require Import pos vec.
+
+From Undecidability.H10.Fractran 
+  Require Import fractran_defs prime_seq.
+
+From Undecidability.H10.Dio 
+  Require Import dio_logic dio_bounded dio_rt_closure dio_single.
 
 Set Implicit Arguments.
 
@@ -31,20 +37,19 @@ Section fractran_dio.
   Proof.
     intros Hx Hy.
     induction l as [ | (p,q) l IHl ].
-    + apply dio_rel_equiv with (fun _ => False); auto.
-      intros v; rewrite fractran_step_nil_inv; split; tauto.
-    + apply dio_rel_equiv with (1 := fun v => fractran_step_cons_inv p q l (x v) (y v)); auto.
+    + by dio equiv (fun _ => False).
+      abstract (intros v; rewrite fractran_step_nil_inv; split; tauto).
+    + apply dio_rel_equiv with (1 := fun v => fractran_step_cons_inv p q l (x v) (y v)).
+      dio_rel_auto.
   Defined.
 
-  Hint Resolve dio_rel_fractran_step.
+  Hint Resolve dio_rel_fractran_step : dio_rel_db.
 
   (* Hence Fractan step* (refl. trans. closure) is diophantine *)
 
   Theorem dio_rel_fractran_rt l x y : 
                      𝔻P x -> 𝔻P y -> 𝔻R (fun ν => fractran_compute l (x ν) (y ν)).
-  Proof.
-    intros; apply dio_rel_exst, dio_rel_rel_iter; auto.
-  Defined.
+  Proof. intros; apply dio_rel_rt; dio_rel_auto. Defined.
 
   (* Fractran stop is a diophantine relation *)
 
@@ -52,13 +57,13 @@ Section fractran_dio.
   Proof.
     intros Hx.
     induction l as [ | (p,q) l IHl ].
-    + apply dio_rel_equiv with (fun _ => True); auto.
-      intro v; split; auto; intros _ ?.
-      rewrite fractran_step_nil_inv; auto.
-    + apply dio_rel_equiv with (1 := fun v => fractan_stop_cons_inv p q l (x v)); auto.
+    + by dio equiv (fun _ => True).
+      abstract(intro v; split; auto; intros _ ?; rewrite fractran_step_nil_inv; auto).
+    + apply dio_rel_equiv with (1 := fun v => fractan_stop_cons_inv p q l (x v)).
+      dio_rel_auto.
   Defined.
 
-  Hint Resolve dio_rel_fractran_rt dio_rel_fractran_stop.
+  Hint Resolve dio_rel_fractran_rt dio_rel_fractran_stop : dio_rel_db.
 
   (* We start with the case of regular Fractran programs that do not
      contain (_,0) "fractions" *)
@@ -67,17 +72,13 @@ Section fractran_dio.
 
   Theorem FRACTRAN_HALTING_on_diophantine ll x :
                       𝔻P x -> 𝔻R (fun ν => FRACTRAN_HALTING (ll,x ν)).
-  Proof.
-    intros; apply dio_rel_exst, dio_rel_conj; auto.
-  Defined.
+  Proof. intros; dio_rel_auto. Defined.
 
   Theorem FRACTRAN_HALTING_diophantine_0 ll : 𝔻R (fun ν => FRACTRAN_HALTING (ll,ν 0)).
-  Proof.
-    intros; apply FRACTRAN_HALTING_on_diophantine; auto.
-  Defined.
+  Proof. intros; apply FRACTRAN_HALTING_on_diophantine; dio_rel_auto. Defined.
 
   Theorem FRACTRAN_HALTING_diophantine l x : 𝔻R (fun _ => FRACTRAN_HALTING (l,x)).
-  Proof. apply FRACTRAN_HALTING_on_diophantine; auto. Defined.
+  Proof. apply FRACTRAN_HALTING_on_diophantine; dio_rel_auto. Defined.
 
 End fractran_dio.
 
@@ -93,7 +94,7 @@ Qed.
 Theorem FRACTRAN_HALTING_dio_single l x : { e : dio_single nat Empty_set | l /F/ x ↓ <-> dio_single_pred e (fun _ => 0) }.
 Proof.
   generalize (@FRACTRAN_HALTING_on_diophantine l (fun _ => x)); intros H1.
-  spec in H1; auto.
+  spec in H1; dio_rel_auto.
   destruct dio_rel_single with (1 := H1) as ((p,q) & He).
   unfold FRACTRAN_HALTING in He.
   exists (dp_inst_par (fun _ => 0) p, dp_inst_par (fun _ => 0) q).
@@ -121,11 +122,9 @@ Section exp_diophantine.
         * intros (q1 & q2 & H & ? & ?); subst.
           rewrite H, power_expo; auto. }
       apply dio_rel_equiv with (1 := H); clear H.
-      do 2 apply dio_rel_exst.
-      apply dio_rel_conj; auto.
-      apply dio_rel_conj; auto.
+      dio_rel_auto.
       assert (H : dio_rel (fun v => v 0 = exp (S i) (fun2vec (3+j) n v))).
-      { apply IHn; auto. }
+      { apply IHn; dio_rel_auto. }
       revert H; apply dio_rel_equiv.
       intros v; rewrite fun2vec_lift with (f := fun i => v (S i)).
       rewrite fun2vec_lift; simpl; tauto.
@@ -139,25 +138,26 @@ Section exp_diophantine.
 
   Hint Resolve exp_dio.
 
-  Fact exp_diophantine n : 𝔻R (fun ν => ν 0 = ps 1 * exp 1 (fun2vec 0 n (fun x => ν (S x)))).
+  Fact exp_diophantine n : 𝔻P (fun ν => ps 1 * exp 1 (fun2vec 0 n ν)).
   Proof.
-    apply dio_rel_equiv with (fun v => exists y, v 0 = ps 1 * y 
-                                    /\ y = exp 1 (fun2vec 0 n (fun x => v (S x)))).
+    by dio equiv (fun v => exists y, v 0 = ps 1 * y 
+                                  /\ y = exp 1 (fun2vec 0 n (fun x => v (S x)))).
     + intro v; split.
       * exists (exp 1 (fun2vec 0 n (fun x => v (S x)))); auto.
       * intros (y & H1 & <-); auto.
-    + apply dio_rel_exst, dio_rel_conj; auto.
-      apply dio_rel_equiv with (fun v => v 0 = exp 1 (fun2vec 2 n v)); auto.
-      intro; repeat rewrite <- fun2vec_lift; tauto.
+    + apply dio_rel_eq; dio_rel_auto.
+      apply dio_rel_equiv with (fun v => v 0 = exp 1 (fun2vec 3 n v)); dio_rel_auto.
+      intro; repeat rewrite <- fun2vec_lift; simpl; tauto.
   Qed.
 
 End exp_diophantine.
 
-Hint Resolve exp_diophantine.
+Hint Resolve exp_diophantine : dio_rel_db.
 
 Theorem FRACTRAN_HALTING_on_exp_diophantine n l :  
                      𝔻R (fun ν => l /F/ ps 1 * exp 1 (fun2vec 0 n ν) ↓).
 Proof.
-  apply dio_rel_compose with (R := fun x v => l /F/ x ↓); auto.
-  apply FRACTRAN_HALTING_on_diophantine; auto.
+  apply dio_rel_compose with (R := fun x v => l /F/ x ↓).
+  + apply exp_diophantine.
+  + apply FRACTRAN_HALTING_on_diophantine; dio_rel_auto.
 Qed.
